- Somma: G primitiva di $g$ e F primitiva di $f$, G+F è primitiva di $g+f$.
- Prodotto: $\beta F$ è primitiva di $\beta f$.

### Esercizi
1. $f(x)=2cosx+\dfrac{1}{x^3}-\sqrt[3]{x}$
	$F(x)=2sinx-\dfrac{1}{2}x^{-2}-\dfrac{3}{4}x^{\frac{4}{3}}+c$
2. $f(x)=\dfrac{1}{3}cos(4x)$
	$F(x)=\dfrac{1}{12} sin(4x)+c$ 
3. $f(x)=sin(2x+1)$
	$F(x)=-\dfrac{1}{2} cos(2x+1)+c$
4. $f(x)=sin(3x)+e^{5x+1}$
	$F(x)=-\dfrac{1}{3}cos(3x)+\dfrac{1}{5}e^{5x+1}+c$
5. $f(x)=\dfrac{1}{(3x+2)^5}$
	$F(x)=-\dfrac{1}{12}(3x+2)^{-4}+c$

### 